Some progress with allocation in inode proof

external/Goose/github_com/mit_pdos/perennial_examples/inode.v
@@ -2,6 +2,7 @@
 From Perennial.goose_lang Require Import prelude.
 From Perennial.goose_lang Require Import ffi.disk_prelude.
 
+From Goose Require github_com.mit_pdos.perennial_examples.alloc.
 From Goose Require github_com.tchajed.marshal.
 
 Definition MaxBlocks : expr := #511.
@@ -63,40 +64,25 @@ Definition Inode__mkHdr: val :=
     let: "hdr" := marshal.Enc__Finish "enc" in
     "hdr".
 
-Definition AppendStatus: ty := byteT.
-
-Definition AppendOk : expr := #(U8 0).
-
-Definition AppendAgain : expr := #(U8 1).
-
-Definition AppendFull : expr := #(U8 2).
-
 (* Append adds a block to the inode.
 
-   Takes ownership of the disk at a on success.
-
-   Returns:
-   - AppendOk on success and takes ownership of the allocated block.
-   - AppendFull if inode is out of space (and returns the allocated block)
-   - AppendAgain if inode needs a metadata block. Call i.Alloc and try again.
-   	 Returns the allocated block. *)
+   Returns false on failure (if the allocator or inode are out of space) *)
 Definition Inode__Append: val :=
-  rec: "Inode__Append" "i" "a" :=
-    lock.acquire (struct.loadF Inode.S "m" "i");;
-    (if: slice.len (struct.loadF Inode.S "addrs" "i") ≥ MaxBlocks
-    then
-      lock.release (struct.loadF Inode.S "m" "i");;
-      AppendFull
+  rec: "Inode__Append" "i" "b" "allocator" :=
+    let: ("a", "ok") := alloc.Allocator__Reserve "allocator" in
+    (if: ~ "ok"
+    then #false
     else
-      struct.storeF Inode.S "addrs" "i" (SliceAppend uint64T (struct.loadF Inode.S "addrs" "i") "a");;
-      let: "hdr" := Inode__mkHdr "i" in
-      disk.Write (struct.loadF Inode.S "addr" "i") "hdr";;
-      lock.release (struct.loadF Inode.S "m" "i");;
-      AppendOk).
-
-(* Give a block to the inode for metadata purposes.
-
-   Returns true if the block was consumed. *)
-Definition Inode__Alloc: val :=
-  rec: "Inode__Alloc" "i" "a" :=
-    #false.
+      disk.Write "a" "b";;
+      lock.acquire (struct.loadF Inode.S "m" "i");;
+      (if: slice.len (struct.loadF Inode.S "addrs" "i") ≥ MaxBlocks
+      then
+        alloc.Allocator__Free "allocator" "a";;
+        lock.release (struct.loadF Inode.S "m" "i");;
+        #false
+      else
+        struct.storeF Inode.S "addrs" "i" (SliceAppend uint64T (struct.loadF Inode.S "addrs" "i") "a");;
+        let: "hdr" := Inode__mkHdr "i" in
+        disk.Write (struct.loadF Inode.S "addr" "i") "hdr";;
+        lock.release (struct.loadF Inode.S "m" "i");;
+        #true)).
